refinedVST/typing/base.v
@@ -1,5 +1,6 @@
+From stdpp Require Import coPset.
 From VST.lithium Require Export syntax definitions.
-From VST Require Export floyd.proofauto shared.dshare.
+From VST Require Export floyd.core_base shared.dshare.
 
 Class CoPsetFact (P : Prop) : Prop := copset_fact : P.
 (* clear for performance reasons as there can be many hypothesis and they should not be needed for the goals which occur *)
